theories/ftlr/ReadSR.v
@@ -1,0 +1,76 @@
+From cap_machine Require Export logrel.
+From iris.proofmode Require Import proofmode.
+From iris.program_logic Require Import weakestpre adequacy lifting.
+From stdpp Require Import base.
+From cap_machine.ftlr Require Import ftlr_base interp_weakening.
+From cap_machine.rules Require Import rules_base rules_ReadSR.
+From cap_machine.proofmode Require Import map_simpl register_tactics.
+From cap_machine Require Import stdpp_extra.
+
+Section fundamental.
+  Context
+    {Σ : gFunctors}
+      {ceriseg: ceriseG Σ}
+      {stsg : STSG Addr region_type Σ} {heapg : heapGS Σ}
+      {sealsg: sealStoreG Σ}
+      {nainv: logrel_na_invs Σ}
+      {MP: MachineParameters}
+  .
+
+  Notation STS := (leibnizO (STS_states * STS_rels)).
+  Notation STS_STD := (leibnizO (STS_std_states Addr region_type)).
+  Notation WORLD := (prodO STS_STD STS).
+  Implicit Types W : WORLD.
+
+  Notation D := (WORLD -n> (leibnizO Word) -n> iPropO Σ).
+  Notation R := (WORLD -n> (leibnizO Reg) -n> iPropO Σ).
+  Implicit Types w : (leibnizO Word).
+  Implicit Types interp : (D).
+
+  Lemma readsr_case (W : WORLD) (regs : leibnizO Reg)
+    (p p' : Perm) (g : Locality) (b e a : Addr)
+    (w : Word) (ρ : region_type) (dst : RegName) (src : SRegName) (P:D) :
+    ftlr_instr W regs p p' g b e a w (ReadSR dst src) ρ P.
+  Proof.
+    intros Hp Hsome HcorrectPC Hbae Hfp HO Hpers Hpwl Hregion Hnotrevoked Hnotfrozen Hi.
+    iIntros "#IH #Hinv_interp #Hreg #Hinva #Hrcond #Hwcond #Hmono #HmonoV Hw Hsts Hown".
+    iIntros "Hr Hstate Ha HPC Hmap".
+    iInsert "Hmap" PC.
+    destruct (has_sreg_access p) eqn:HpXRS.
+    { iClear "IH Hreg Hinva Hrcond Hwcond Hmono HmonoV Hw Hsts Hown Hr Hstate Ha Hmap".
+      iEval (rewrite !fixpoint_interp1_eq interp1_eq) in "Hinv_interp".
+      destruct (isO p) eqn: HnO.
+      { destruct Hp as [Hexec _]
+        ; eapply executeAllowed_nonO in Hexec
+        ; congruence.
+      }
+      destruct (isE p) eqn:HpnotE.
+      { destruct Hp as [Hexec _]
+        ; eapply executeAllowed_nonE in Hexec
+        ; eauto
+        ; congruence.
+      }
+      destruct (isESR p) eqn:HpnotESR.
+      { destruct Hp as [Hexec _]
+        ; eapply executeAllowed_nonESR in Hexec
+        ; eauto
+        ; congruence.
+      }
+      destruct (has_sreg_access p) eqn:HpXRS'; first done.
+      congruence.
+    }
+
+    iApply (wp_ReadSR with "[$Ha $Hmap]"); eauto.
+    { simplify_map_eq; auto. }
+    { rewrite /subseteq /map_subseteq. intros rr _.
+      apply elem_of_dom. apply lookup_insert_is_Some'; eauto. }
+    { by rewrite HpXRS. }
+
+    iIntros "!>" (regs' retv). iDestruct 1 as (HSpec) "[Ha Hmap]".
+    destruct HSpec; cycle 1.
+    - iApply wp_pure_step_later; auto. iNext; iIntros "_".
+      iApply wp_value; auto. iIntros; discriminate.
+    - by simplify_map_eq.
+  Qed.
+
+End fundamental.
