theories/rules/rules_ReadSR.v
@@ -1,0 +1,192 @@
+From iris.base_logic Require Export invariants gen_heap.
+From iris.program_logic Require Export weakestpre ectx_lifting.
+From iris.proofmode Require Import proofmode.
+From iris.algebra Require Import frac.
+From cap_machine Require Export rules_base.
+
+Section cap_lang_rules.
+  Context `{MP: MachineParameters}.
+  Context `{ceriseg: ceriseG Σ}.
+  Implicit Types P Q : iProp Σ.
+  Implicit Types σ : ExecConf.
+  Implicit Types c : cap_lang.expr.
+  Implicit Types a b : Addr.
+  Implicit Types r : RegName.
+  Implicit Types v : cap_lang.val.
+  Implicit Types w : Word.
+  Implicit Types reg : gmap RegName Word.
+  Implicit Types sreg : gmap SRegName Word.
+  Implicit Types ms : gmap Addr Word.
+
+  Inductive ReadSR_failure (regs: Reg) (sregs : SReg) (dst: RegName) (src: SRegName) :=
+  | ReadSR_fail_nonxrs p g b e a:
+      regs !! PC = Some (WCap p g b e a) →
+      has_sreg_access p = false ->
+      ReadSR_failure regs sregs dst src
+  | ReadSR_fail_incrPC p g b e a w:
+      regs !! PC = Some (WCap p g b e a) →
+      sregs !! src = Some w →
+      incrementPC (<[ dst := w ]> regs) = None →
+      ReadSR_failure regs sregs dst src
+  .
+
+  Inductive ReadSR_spec
+  (regs: Reg) (sregs: SReg) (dst: RegName) (src: SRegName) (regs': Reg)
+    : cap_lang.val -> Prop :=
+  | ReadSR_spec_success p g b e a w:
+      regs !! PC = Some (WCap p g b e a) →
+      has_sreg_access p = true ->
+      sregs !! src = Some w →
+      incrementPC (<[ dst := w ]> regs) = Some regs' →
+      ReadSR_spec regs sregs dst src regs' NextIV
+  | ReadSR_spec_failure:
+      ReadSR_failure regs sregs dst src →
+      ReadSR_spec regs sregs dst src regs' FailedV.
+
+  Lemma wp_ReadSR Ep pc_p pc_g pc_b pc_e pc_a w dst src regs sregs :
+    decodeInstrW w = ReadSR dst src ->
+    isCorrectPC (WCap pc_p pc_g pc_b pc_e pc_a) →
+    regs !! PC = Some (WCap pc_p pc_g pc_b pc_e pc_a) →
+    regs_of (ReadSR dst src) ⊆ dom regs →
+    (if (has_sreg_access pc_p)
+    then sregs_of (ReadSR dst src) ⊆ dom sregs
+    else True) →
+    {{{ ▷ pc_a ↦ₐ w ∗
+        ▷ ([∗ map] k↦y ∈ regs, k ↦ᵣ y) ∗
+        ▷ ([∗ map] k↦y ∈ sregs, k ↦ₛᵣ y)
+    }}}
+      Instr Executable @ Ep
+    {{{ regs' retv, RET retv;
+        ⌜ ReadSR_spec regs sregs dst src regs' retv ⌝ ∗
+        pc_a ↦ₐ w ∗
+        ([∗ map] k↦y ∈ regs', k ↦ᵣ y) ∗
+        ([∗ map] k↦y ∈ sregs, k ↦ₛᵣ y)
+    }}}.
+  Proof.
+    iIntros (Hinstr Hvpc HPC Dregs Dsregs φ) "(>Hpc_a & >Hmap & >Hsmap) Hφ".
+    iApply wp_lift_atomic_base_step_no_fork; auto.
+    iIntros (σ1 ns l1 l2 nt) "[ [Hr Hsr] Hm ] /=". destruct σ1 as [ [r sr] m]; cbn.
+    iDestruct (gen_heap_valid_inclSepM with "Hr Hmap") as %Hregs.
+    iDestruct (gen_heap_valid_inclSepM with "Hsr Hsmap") as %Hsregs.
+    have ? := lookup_weaken _ _ _ _ HPC Hregs.
+    iDestruct (@gen_heap_valid with "Hm Hpc_a") as %Hpc_a; auto.
+    iModIntro. iSplitR. by iPureIntro; apply normal_always_base_reducible.
+    iNext. iIntros (e2 σ2 efs Hpstep).
+    apply prim_step_exec_inv in Hpstep as (-> & -> & (c & -> & Hstep)).
+    iIntros "_".
+    iSplitR; auto. eapply step_exec_inv in Hstep; eauto.
+    unfold exec in Hstep.
+
+    specialize (indom_regs_incl _ _ _ Dregs Hregs) as Hri. unfold regs_of in Hri.
+    destruct (Hri dst) as [wdst [H'dst Hdst]]. by set_solver+.
+
+    destruct (has_sreg_access pc_p) eqn:Hxsr; cycle 1.
+    { cbn in Hstep. rewrite Hxsr in Hstep.
+      simplify_eq.
+      iFailWP "Hφ" ReadSR_fail_nonxrs.
+    }
+
+    specialize (indom_sregs_incl _ _ _ Dsregs Hsregs) as Hsri. unfold sregs_of in Hsri.
+    destruct (Hsri src) as [wsrc [H'src Hsrc]]. by set_solver+.
+
+    assert (exec_opt (ReadSR dst src) pc_p (r, sr, m) = updatePC (update_reg (r, sr, m) dst wsrc)) as HH.
+    { by cbn; rewrite Hsrc Hxsr /=. }
+    rewrite HH in Hstep. rewrite /update_reg /= in Hstep.
+
+    destruct (incrementPC (<[ dst := wsrc ]> regs)) as [regs'|] eqn:Hregs'
+    ; pose proof Hregs' as H'regs'; cycle 1.
+    { apply incrementPC_fail_updatePC with (sregs:=sr) (m:=m) in Hregs'.
+      eapply updatePC_fail_incl with (sregs':=sr) (m':=m) in Hregs'.
+      2: by apply lookup_insert_is_Some'; eauto.
+      2: by apply insert_mono; eauto.
+      rewrite Hregs' in Hstep. simplify_pair_eq.
+      iFailWP "Hφ" ReadSR_fail_incrPC.
+    }
+
+    eapply (incrementPC_success_updatePC _ sr m) in Hregs'
+      as (p' & g' & b' & e' & a'' & a''' & a_pc' & HPC'' & HuPC & ->).
+    eapply updatePC_success_incl with (sregs':=sr) (m':=m) in HuPC. 2: by eapply insert_mono; eauto.
+    rewrite HuPC in Hstep. simplify_pair_eq. iFrame.
+    iMod ((gen_heap_update_inSepM _ _ dst) with "Hr Hmap") as "[Hr Hmap]"; eauto.
+    iMod ((gen_heap_update_inSepM _ _ PC) with "Hr Hmap") as "[Hr Hmap]"; eauto.
+    iFrame. iModIntro. iApply "Hφ". iFrame. iPureIntro. econstructor; eauto.
+  Qed.
+
+  Lemma wp_readsr_success E pc_p pc_g pc_b pc_e pc_a pc_a' w dst wdst src wsrc :
+    decodeInstrW w = ReadSR dst src →
+    isCorrectPC (WCap pc_p pc_g pc_b pc_e pc_a) →
+    has_sreg_access pc_p = true →
+    (pc_a + 1)%a = Some pc_a' →
+
+    {{{ ▷ PC ↦ᵣ WCap pc_p pc_g pc_b pc_e pc_a
+        ∗ ▷ pc_a ↦ₐ w
+        ∗ ▷ dst ↦ᵣ wdst
+        ∗ ▷ src ↦ₛᵣ wsrc }}}
+      Instr Executable @ E
+      {{{ RET NextIV;
+          PC ↦ᵣ WCap pc_p pc_g pc_b pc_e pc_a'
+          ∗ pc_a ↦ₐ w
+          ∗ dst ↦ᵣ wsrc
+          ∗ src ↦ₛᵣ wsrc }}}.
+  Proof.
+    iIntros (Hinstr Hvpc Hxsr Hpca' ϕ) "(>HPC & >Hpc_a & >Hdst & >Hsrc) Hφ".
+    iDestruct (map_of_regs_2 with "HPC Hdst") as "[Hmap %]".
+    iDestruct (map_of_sregs_1 with "Hsrc") as "Hsmap".
+    iApply (wp_ReadSR with "[$Hmap $Hsmap Hpc_a]"); eauto; simplify_map_eq; eauto.
+    - by unfold regs_of; rewrite !dom_insert; set_solver+.
+    - by unfold sregs_of; rewrite Hxsr !dom_insert; set_solver+.
+    - iNext. iIntros (regs' retv) "(#Hspec & Hpc_a & Hmap & Hsmap)". iDestruct "Hspec" as %Hspec.
+
+    destruct Hspec as [| Hfail].
+    { (* Success *)
+      iApply "Hφ". iFrame. incrementPC_inv; simplify_map_eq.
+      rewrite (insert_commute _ PC dst) // insert_insert (insert_commute _ PC dst) // insert_insert.
+      iDestruct (regs_of_map_2 with "Hmap") as "(?&?&?)"; eauto; iFrame.
+      iDestruct (sregs_of_map_1 with "Hsmap") as "?"; eauto; iFrame.
+    }
+    { (* Failure (contradiction) *)
+      destruct Hfail.
+      - simplify_map_eq; eauto; congruence.
+      - incrementPC_inv; simplify_map_eq; eauto.
+        congruence.
+    }
+  Qed.
+
+  Lemma wp_readsr_success_toPC E pc_p pc_g pc_b pc_e pc_a w src p g b e a a':
+    decodeInstrW w = ReadSR PC src →
+    isCorrectPC (WCap pc_p pc_g pc_b pc_e pc_a) →
+    has_sreg_access pc_p = true →
+    (a + 1)%a = Some a' →
+
+    {{{ ▷ PC ↦ᵣ WCap pc_p pc_g pc_b pc_e pc_a
+        ∗ ▷ pc_a ↦ₐ w
+        ∗ ▷ src ↦ₛᵣ WCap p g b e a }}}
+      Instr Executable @ E
+      {{{ RET NextIV;
+          PC ↦ᵣ WCap p g b e a'
+          ∗ pc_a ↦ₐ w
+          ∗ src ↦ₛᵣ WCap p g b e a }}}.
+  Proof.
+    iIntros (Hinstr Hvpc Hxsr Hpca' ϕ) "(>HPC & >Hpc_a & >Hsrc) Hφ".
+    iDestruct (map_of_regs_1 with "HPC") as "Hmap".
+    iDestruct (map_of_sregs_1 with "Hsrc") as "Hsmap".
+    iApply (wp_ReadSR with "[$Hmap $Hsmap Hpc_a]"); eauto; simplify_map_eq; eauto.
+    { by unfold sregs_of; rewrite Hxsr !dom_insert; set_solver+. }
+    iNext. iIntros (regs' retv) "(#Hspec & Hpc_a & Hmap & Hsmap)". iDestruct "Hspec" as %Hspec.
+
+    destruct Hspec as [|Hfail].
+    { (* Success *)
+      iApply "Hφ". iFrame. incrementPC_inv; simplify_map_eq.
+      rewrite !insert_insert.
+      iDestruct (regs_of_map_1 with "Hmap") as "?"; eauto; iFrame.
+      iDestruct (sregs_of_map_1 with "Hsmap") as "?"; eauto; iFrame.
+    }
+    { (* Failure (contradiction) *)
+      destruct Hfail.
+      - simplify_map_eq; eauto; congruence.
+      - incrementPC_inv; simplify_map_eq; eauto.
+        congruence.
+    }
+  Qed.
+
+End cap_lang_rules.
