theories/rules/rules_Seal.v
@@ -65,8 +65,7 @@ Section cap_lang_rules.
   Proof.
     iIntros (Hinstr Hvpc HPC Dregs φ) "(>Hpc_a & >Hmap) Hφ".
     iApply wp_lift_atomic_base_step_no_fork; auto.
-    iIntros (σ1 ns l1 l2 nt) "Hσ1 /=". destruct σ1; simpl.
-    iDestruct "Hσ1" as "[Hr Hm]".
+    iIntros (σ1 ns l1 l2 nt) "[ [Hr Hsr] Hm ] /=". destruct σ1 as [ [r sr] m]; cbn.
     iDestruct (gen_heap_valid_inclSepM with "Hr Hmap") as %Hregs.
     have ? := lookup_weaken _ _ _ _ HPC Hregs.
     iDestruct (@gen_heap_valid with "Hm Hpc_a") as %Hpc_a; auto.
@@ -86,7 +85,7 @@ Section cap_lang_rules.
     (* Now we start splitting on the different cases in the Seal spec, and prove them one at a time *)
      destruct (is_sealr r1v) eqn:Hr1v.
      2:{ (* Failure: r2 is not a sealrange *)
-       assert (c = Failed ∧ σ2 = (r, m)) as (-> & ->).
+       assert (c = Failed ∧ σ2 = (r, sr, m)) as (-> & ->).
        {
          unfold is_sealr in Hr1v.
          destruct_word r1v; by simplify_pair_eq.
@@ -97,7 +96,7 @@ Section cap_lang_rules.
 
      destruct (is_sealb r2v) eqn:Hr2v.
      2:{ (* Failure: r2 is not a sealrange *)
-       assert (c = Failed ∧ σ2 = (r, m)) as (-> & ->).
+       assert (c = Failed ∧ σ2 = (r, sr, m)) as (-> & ->).
        {
          unfold is_sealed in Hr2v.
          destruct_word r2v; by simplify_pair_eq.
@@ -129,7 +128,7 @@ Section cap_lang_rules.
 
      (* Success *)
      rewrite /update_reg /= in Hstep.
-     eapply (incrementPC_success_updatePC _ m) in Hregs'
+     eapply (incrementPC_success_updatePC _ sr m) in Hregs'
        as (p1 & g1 & b1 & e1 & a1 & a_pc1 & HPC'' & Ha_pc' & HuPC & ->).
      eapply updatePC_success_incl in HuPC. 2: by eapply insert_mono.
      rewrite HuPC in Hstep; clear HuPC; inversion Hstep; clear Hstep; subst c σ2. cbn.
